modified correctness spec of max prefix to allow for DFA approach

lexer.v
@@ -46,9 +46,17 @@ Definition transition : Sigma -> State -> State := derivative.
 Definition accepts : String -> State -> bool := exp_matchb.
 Definition accepting : State -> bool:= nullable.
 Definition init_state (r : regex) : State := r.
-Definition absorbing_state := EmptySet.
+Definition init_state_inv (fsm : State) : regex := fsm.
+
+Lemma invert_init_correct : forall(r : regex),
+    init_state_inv (init_state r) = r.
+Proof.
+  intros r. unfold init_state. unfold init_state_inv. reflexivity.
+Qed.
+
 (* in eRule, the State would be the initial state of the machine after converting from regex *)
 Definition eRule : Type := String * regex * State.
+Definition absorbing_state := EmptySet.
 Definition eeToken : Type := eRule * String * String.
 Definition eeLexemes : Type := list eeToken.
 
@@ -207,6 +215,12 @@ Inductive is_prefix : String -> String -> Prop :=
 
 Notation "p ++_= s" := (is_prefix p s) (at level 80).
 
+Lemma nil_is_prefix : forall(xs : String),
+    [] ++_= xs.
+Proof.
+  intros xs. apply pref_def. exists xs. reflexivity.
+Qed.
+
 Lemma app_head_prefix : forall(xs ys : String),
     xs ++_= xs ++ ys.
 Proof.
@@ -254,21 +268,53 @@ Proof.
       * apply H2.
 Qed.
 
+Inductive eq_models : State -> regex -> Prop :=
+| SReq (fsm : State) (r : regex)
+       (H1 : forall(s : String), true = accepts s fsm <-> exp_match s r) :
+    eq_models fsm r.
 
-(* Need to replace exp_match with something more general to States *)
-(* maybe we can pass the regex AND the State here and add a hypothesis about their equivalence *)
+Lemma accepts_matches : forall(s : String) (fsm : State),
+    true = accepts s fsm <-> exp_match s (init_state_inv fsm).
+Proof.
+  intros s fsm. apply match_iff_matchb.
+Qed.
+
+Lemma inv_eq_model : forall(fsm : State),
+    eq_models fsm (init_state_inv fsm).
+Proof.
+  intros fsm. apply SReq. intros s. apply match_iff_matchb.
+Qed.
+
+Lemma accepts_nil: forall(fsm : State),
+    accepting fsm = accepts [] fsm.
+Proof.
+  intros fsm. reflexivity.
+Qed.
+
+Inductive re_no_max_pref : String -> State -> regex -> Prop :=
+| re_MP0 (s : String) (fsm : State) (r : regex)
+      (H0 : eq_models fsm r)
+      (H1 : forall cand, cand ++_= s -> ~(exp_match cand r)) :
+    re_no_max_pref s fsm r.
+
+Inductive re_max_pref : String -> State -> regex -> String -> Prop :=
+| re_MP1 (s p : String) (fsm : State) (r : regex)
+         (H0 : eq_models fsm r)
+         (H1 : p ++_= s)
+         (H2 : exp_match p r)
+         (H3 : forall(cand : String), cand ++_= s
+                                 -> ((length cand) <= (length p)) \/ ~(exp_match cand r)) :
+    re_max_pref s fsm r p.
+
 Inductive no_max_pref : String -> State -> Prop :=
-| MP0 (s : String) (r : State)
-         (H1 : forall cand, cand ++_= s -> ~(exp_match cand r)) :
-    no_max_pref s r.
+| MP0 (s : String) (fsm : State)
+      (H1 : exists(r : regex), re_no_max_pref s fsm r) : 
+    no_max_pref s fsm.
 
 Inductive max_pref : String -> State -> String -> Prop :=
-| MP1 (s : String) (r : State) (p : String)
-      (H1 : p ++_= s)
-      (H2 : exp_match p r)
-      (H3 : forall(cand : String), cand ++_= s
-                              -> ((length cand) <= (length p)) \/ ~(exp_match cand r)) :
-    max_pref s r p.
+| MP1 (s p : String) (fsm : State)
+      (H1 : exists(r : regex), re_max_pref s fsm r p) : 
+    max_pref s fsm p.
 
 Lemma false_not_true : forall(b : bool),
     b = false <-> not(b = true).
@@ -282,27 +328,30 @@ Proof.
     + reflexivity.
 Qed.
 
-Theorem max_pref_correct_None : forall(code : String) (fsm : State),
-    no_max_pref code fsm <-> None = max_pref_fn code fsm.
+Theorem re_max_pref_correct__None : forall(code : String) (fsm : State),
+    re_no_max_pref code fsm (init_state_inv fsm)
+    <-> None = max_pref_fn code fsm.
 Proof.
   intros code fsm. split.
   {
     generalize dependent fsm; induction code; intros fsm H.
     - simpl. inv H. specialize (H1 []). assert (A : [] ++_= []).
-      { apply pref_def. exists []. reflexivity. }
+      { apply nil_is_prefix. }
       apply H1 in A. clear H1. destruct (accepting fsm) eqn:E.
       + exfalso. unfold not in A. destruct A. apply nullable_bridge.
         symmetry. unfold accepting in E. apply E.
       + reflexivity.
     - specialize (IHcode (transition a fsm)). inv H.
-      assert (A0 : no_max_pref code (transition a fsm)).
+      assert (A0 : re_no_max_pref code (init_state_inv (transition a fsm)) (transition a fsm)).
       {
-        apply MP0. intros cand H. specialize (H1 (a :: cand)).
-        assert (A1 : a :: cand ++_= a :: code).
-        { apply pref_def. inv H. destruct H0. exists x. rewrite <- H. reflexivity. }
-        apply H1 in A1. unfold not. intros C. unfold not in A1. destruct A1.
-        apply match_iff_matchb. apply match_iff_matchb in C. simpl. unfold transition in C.
-        apply C.
+        apply re_MP0.
+        - apply inv_eq_model.
+        - intros cand H. specialize (H1 (a :: cand)).
+          assert (A1 : a :: cand ++_= a :: code).
+          { apply pref_def. inv H. destruct H2. exists x. rewrite <- H. reflexivity. }
+          apply H1 in A1. unfold not. intros C. unfold not in A1. destruct A1.
+          apply match_iff_matchb. apply match_iff_matchb in C. simpl. unfold transition in C.
+          apply C.
       }
       apply IHcode in A0.
       simpl.
@@ -316,7 +365,7 @@ Proof.
       assert (A2 : accepting fsm = false).
       {
         specialize (H1 []). assert (A3 : [] ++_= a :: code).
-        { apply pref_def. exists (a :: code). reflexivity. }
+        { apply nil_is_prefix. }
         apply H1 in A3. apply false_not_true. unfold not. intros C.
         unfold not in A3. destruct A3. apply nullable_bridge. unfold accepting in C.
         symmetry. apply C.
@@ -325,53 +374,60 @@ Proof.
   }
   {
     generalize dependent fsm; induction code; intros fsm H.
-    - apply MP0. intros cand H0. simpl in H.
-      assert (A0 : accepting fsm = false).
-      {
-        destruct (accepting fsm).
-        - discriminate.
-        - reflexivity.
-      }
-      assert (A1 : cand = []).
-      {
-        destruct cand.
-        - reflexivity.
-        - inv H0. destruct H1. discriminate.
-      } 
-      unfold not. intros C. rewrite A1 in C. apply nullable_bridge in C.
-      unfold accepting in A0. rewrite A0 in C. discriminate.
-    - specialize (IHcode (transition a fsm)).
-      apply MP0. intros cand H0. simpl in H. destruct (max_pref_fn code (transition a fsm)).
-      + destruct p. discriminate.
-      + assert (A0 : accepting (transition a fsm) = false).
+    - apply re_MP0.
+      + apply inv_eq_model.
+      + intros cand H0. simpl in H.
+        assert (A0 : accepting fsm = false).
         {
-          destruct (accepting (transition a fsm)).
+          destruct (accepting fsm).
           - discriminate.
           - reflexivity.
         }
-        assert (A1 : accepting fsm = false).
+        assert (A1 : cand = []).
         {
-          destruct (accepting fsm).
-          - rewrite A0 in H. discriminate.
+          destruct cand.
           - reflexivity.
-        }
-        destruct cand.
-        * intros C. apply nullable_bridge in C. unfold accepting in A1.
-          rewrite A1 in C. discriminate.
-        * destruct (Sigma_dec a s).
-          -- rewrite <- e. destruct cand.
-             ++ unfold not. intros C. apply match_iff_matchb in C. simpl in C.
-                unfold accepting in A0. unfold transition in A0.
-                rewrite A0 in C. discriminate.
-             ++ assert (A2 : no_max_pref code (transition a fsm)).
-                { apply IHcode. reflexivity. }
-                inv A2. specialize (H1 (s0 :: cand)). inv H0. destruct H2. injection H0.
-                intros I1. assert (A3 :  s0 :: cand ++_= code).
-                { apply pref_def. exists x. apply I1. }
-                apply H1 in A3. unfold not. intros C. unfold not in A3. destruct A3.
-                apply match_iff_matchb. apply match_iff_matchb in C.
-                simpl. simpl in C. apply C.
-          -- inv H0. destruct H1. injection H0. intros I1 I2. rewrite I2 in n. contradiction.
+          - inv H0. destruct H1. discriminate.
+        } 
+        unfold not. intros C. rewrite A1 in C. rewrite accepts_nil in A0.
+        apply accepts_matches in C. rewrite A0 in C. discriminate.
+    - specialize (IHcode (transition a fsm)).
+      apply re_MP0.
+      { apply inv_eq_model. }
+      {
+        intros cand H0. simpl in H. destruct (max_pref_fn code (transition a fsm)).
+        + destruct p. discriminate.
+        + assert (A0 : accepting (transition a fsm) = false).
+          {
+            destruct (accepting (transition a fsm)).
+            - discriminate.
+            - reflexivity.
+          }
+          assert (A1 : accepting fsm = false).
+          {
+            destruct (accepting fsm).
+            - rewrite A0 in H. discriminate.
+            - reflexivity.
+          }
+          destruct cand.
+          * intros C. rewrite accepts_nil in A1. apply accepts_matches in C.
+            rewrite A1 in C. discriminate.
+          * destruct (Sigma_dec a s).
+            -- rewrite <- e. destruct cand.
+               ++ unfold not. intros C. apply accepts_matches in C. simpl in C.
+                  unfold accepting in A0. unfold transition in A0.
+                  rewrite A0 in C. discriminate.
+               ++ assert (A2 : re_no_max_pref code (init_state_inv (transition a fsm))
+                                              (transition a fsm)).
+                  { apply IHcode. reflexivity. }
+                  inv A2. specialize (H2 (s0 :: cand)). inv H0. destruct H3. injection H0.
+                  intros I1. assert (A3 :  s0 :: cand ++_= code).
+                  { apply pref_def. exists x. apply I1. }
+                  apply H2 in A3. unfold not. intros C. unfold not in A3. destruct A3.
+                  apply match_iff_matchb. apply match_iff_matchb in C.
+                  simpl. simpl in C. apply C.
+            -- inv H0. destruct H1. injection H0. intros I1 I2. rewrite I2 in n. contradiction.
+      }
   }
 Qed.
 
@@ -401,15 +457,16 @@ Proof.
         -- discriminate.
 Qed.
 
-Theorem max_pref_correct_Some : forall(code p : String) (fsm : State),
-    max_pref code fsm p <-> exists(q : String), Some (p, q) = max_pref_fn code fsm.
+Theorem re_max_pref_correct__Some : forall(code p : String) (fsm : State),
+    re_max_pref code fsm (init_state_inv fsm) p
+    <-> exists(q : String), Some (p, q) = max_pref_fn code fsm.
 Proof.
   induction code.
   {
     intros p fsm. split; intros H.
     - exists []. simpl. assert (A0 : p = []).
       {
-        inv H. inv H1. destruct H0. destruct x.
+        inv H. inv H1. destruct H4. destruct x.
         - rewrite nil_right in H. apply H.
         - destruct p.
           + reflexivity.
@@ -417,9 +474,10 @@ Proof.
       }
       destruct (accepting fsm) eqn:E0.
       + rewrite A0. reflexivity.
-      + inv H. apply nullable_bridge in H2. unfold accepting in E0.
+      + inv H. rewrite accepts_nil in E0. apply accepts_matches in H2.
         rewrite E0 in H2. discriminate.
-    - destruct H. apply MP1.
+    - destruct H. apply re_MP1.
+      + apply inv_eq_model.
       + apply max_pref_fn_splits in H. symmetry in H.
         apply pref_def. exists x. apply H.
       + apply max_pref_matches in H. apply H.
@@ -448,11 +506,11 @@ Proof.
           { exists s0. apply E0. }
           apply IHcode in Ae. inv Ae.
           assert (Ap : a :: s ++_= a :: code).
-          { apply cons_prefix. split. reflexivity. apply H0. }
+          { apply cons_prefix. split. reflexivity. apply H5. }
           apply H3 in Ap. destruct Ap.
           -- simpl in H. omega.
           -- exfalso. unfold not in H. destruct H.
-             apply match_iff_matchb. apply match_iff_matchb in H4. simpl. apply H4.
+             apply accepts_matches. simpl. apply accepts_matches in H6. apply H6.
         * assert (A0 : accepting (transition a fsm) = false).
           {
             destruct code.
@@ -467,9 +525,9 @@ Proof.
                   -- discriminate.
                   -- reflexivity.
           }
-          rewrite A0. apply nullable_bridge in H2. unfold accepting. rewrite <- H2.
-          reflexivity.
-      + inv H. inv H1. destruct H0. injection H.
+          rewrite A0. apply accepts_matches in H2. rewrite <- accepts_nil in H2.
+          rewrite <- H2. reflexivity.
+      + inv H. inv H1. destruct H4. injection H.
         intros I1 I2. clear H. exists x. subst s.
         assert (Ap : p ++_= code).
         { apply pref_def. exists x. apply I1. }
@@ -477,27 +535,27 @@ Proof.
         * destruct p0.
           assert (Ae : exists q, Some (s, q) = max_pref_fn code (transition a fsm)).
           { exists s0. apply E0. }
-          apply IHcode in Ae. inv Ae. inv H1. destruct H5. apply max_pref_fn_splits in E0.
+          apply IHcode in Ae. inv Ae. inv H4. destruct H7. apply max_pref_fn_splits in E0.
           (* Want to show p = s *)
           assert (A0 : p ++_= p ++ x).
           { apply pref_def. exists x. reflexivity. }
           assert (A1 : a :: s ++_= a :: p ++ x).
           { apply pref_def. exists x0. rewrite <- H. reflexivity. }
-          apply H3 in A1. apply H4 in A0.
+          apply H3 in A1. apply H6 in A0.
           (* should follow that p and s0 are prefixes of the same length and thus equal *)
           assert (A0' : length p <= length s).
           {
             destruct A0.
-            - apply H1.
-            - exfalso. destruct H1. apply match_iff_matchb in H2. simpl in H2.
-              apply match_iff_matchb. apply H2.
+            - apply H4.
+            - exfalso. destruct H4. apply accepts_matches in H2.
+              apply accepts_matches. simpl in H2. apply H2.
           }
           assert (A1' : length s <= length p).
           {
             destruct A1.
-            - simpl in H1. omega.
-            - exfalso. destruct H1. apply match_iff_matchb in H0.
-              apply match_iff_matchb. simpl. apply H0.
+            - simpl in H4. omega.
+            - exfalso. destruct H4. apply accepts_matches in H5.
+              apply accepts_matches. simpl. apply H5.
           }
           assert (A : length p = length s).
           { omega. }
@@ -507,18 +565,19 @@ Proof.
           -- rewrite A. rewrite A in E0. apply app_inv_head in E0. rewrite E0. reflexivity.
           -- apply As.
           -- apply Ap.
-        * apply max_pref_correct_None in E0. inv E0.
+        * apply re_max_pref_correct__None in E0. inv E0.
           assert (A0 : p = []).
           {
             assert (A1 : p ++_= p ++ x).
             { apply pref_def. exists x. reflexivity. }
-            apply H1 in A1. unfold not in A1. destruct A1.
-            apply match_iff_matchb. apply match_iff_matchb in H2. simpl in H2. subst. apply H2.
+            apply H4 in A1. unfold not in A1. destruct A1. apply accepts_matches.
+            apply accepts_matches in H2. simpl in H2. apply H2.
           }
           assert (A1 : accepting (transition a fsm) = true).
-          { rewrite A0 in H2. apply match_iff_matchb in H2. simpl in H2. symmetry. apply H2. }
+          { rewrite A0 in H2. apply accepts_matches in H2. simpl in H2. symmetry. apply H2. }
           rewrite A1. rewrite A0. reflexivity.
-    - destruct H. apply MP1.
+    - destruct H. apply re_MP1.
+      + apply inv_eq_model.
       + apply max_pref_fn_splits in H. apply pref_def. exists x. symmetry. apply H.
       + apply max_pref_matches in H. apply H.
       + intros cand Hpref. destruct p.
@@ -528,14 +587,15 @@ Proof.
           -- destruct (accepting (transition a fsm)) eqn:E1.
              ++ discriminate.
              ++ destruct (accepting fsm) eqn:E2.
-                ** symmetry in E0. apply max_pref_correct_None in E0. inv E0. destruct cand.
+                ** symmetry in E0. apply re_max_pref_correct__None in E0. inv E0. destruct cand.
                    { left. omega. }
-                   { right. inv Hpref. destruct H0. injection H0. intros I1 I2.
+                   {
+                     right. inv Hpref. destruct H2. injection H2. intros I1 I2.
                      unfold not. intros C. assert (A : cand ++_= code).
                      { apply pref_def. exists x0. apply I1. }
                      apply H1 in A. unfold not in A. destruct A.
-                     apply match_iff_matchb in C. simpl in C. subst a.
-                     apply match_iff_matchb. apply C.
+                     apply accepts_matches in C. simpl in C. subst a.
+                     apply accepts_matches. apply C.
                    }
                 ** discriminate.
         * simpl in H.
@@ -545,21 +605,45 @@ Proof.
              { exists s1. apply E0. }
              apply IHcode in Ae. inv Ae. destruct cand.
              ++ left. simpl. omega.
-             ++ inv Hpref. destruct H0. injection H0. intros I1 I2. subst s.
+             ++ inv Hpref. destruct H4. injection H4. intros I1 I2. subst s.
                 assert (Apref : cand ++_= code).
                 { apply pref_def. exists x. apply I1. }
                 apply H3 in Apref. destruct Apref.
                 ** left. simpl. omega.
-                ** right. intros C. destruct H4. apply match_iff_matchb in C. simpl in C.
-                   apply match_iff_matchb. apply C.
-          -- apply max_pref_correct_None in E0. inv E0.
+                ** right. intros C. destruct H5. apply accepts_matches in C. simpl in C.
+                   apply accepts_matches. apply C.
+          -- apply re_max_pref_correct__None in E0. inv E0.
              assert (A0 : accepting (transition a fsm) = true).
              {
                destruct (accepting (transition a fsm)); destruct (accepting fsm);
                  try(reflexivity); try(discriminate).
              }
              assert (A1 : [] ++_= code).
-             { apply pref_def. exists code. reflexivity. }
-             apply H1 in A1. destruct A1. apply nullable_bridge. symmetry. apply A0.
+             { apply nil_is_prefix. }
+             apply H1 in A1. destruct A1. apply accepts_matches. rewrite <- accepts_nil.
+             symmetry. apply A0.
   }
+Qed.
     
+Theorem max_pref_correct__None : forall(code : String) (fsm : State),
+    no_max_pref code fsm
+    <-> None = max_pref_fn code fsm.
+Proof.
+  intros code fsm. split; intros H.
+  - admit. (* oops, this case doesn't follow easily from the previous theorem.
+              I think I need to make the previous theorem an if and then reuse the other
+              side of the iff to prove this *)
+  - apply re_max_pref_correct__None in H. apply MP0. exists (init_state_inv fsm). apply H.
+Admitted.
+    
+Theorem max_pref_correct__Some : forall(code p : String) (fsm : State),
+    max_pref code fsm p
+    <-> exists(q : String), Some (p, q) = max_pref_fn code fsm.
+Proof.
+  intros code p fsm. split; intros H.
+  - admit. (* oops, this case doesn't follow easily from the previous theorem.
+              I think I need to make the previous theorem an if and then reuse the other
+              side of the iff to prove this *)
+  - apply re_max_pref_correct__Some in H. apply MP1. exists (init_state_inv fsm). apply H.
+Admitted.
+
